coq/theories/bootstrapping/Bootstrapping.v
@@ -14,7 +14,14 @@ Definition compiler_program_imp := to_imp compiler_program_prog.
 
 Compute compiler_program_imp.
 
-Definition get_fun_name (f: FunSyntax.defun): N :=
+Definition compiler_program_asm := match compiler_program_imp with
+| None => []
+| Some p => codegen p
+end.
+
+Eval lazy in compiler_program_asm.
+
+(* Definition get_fun_name (f: FunSyntax.defun): N :=
   match f with
   | FunSyntax.Defun n _ _ => n
   end.
@@ -27,556 +34,49 @@ Definition compiler_funs_imp1 :=
 
 (* Eval lazy in compiler_funs_imp1. *)
 
-Print asm2str_header1_prog.
+Print v2exp_prog.
 Eval lazy in to_cmd (
-  (FunSyntax.Let (FunValues.name_enc "dot_bss")
-    (FunSyntax.Op FunSyntax.Cons
-    [FunSyntax.Const (N_of_ascii "009");
-    FunSyntax.Op FunSyntax.Cons
-    [FunSyntax.Const (N_of_ascii ".");
-    FunSyntax.Op FunSyntax.Cons
-    [FunSyntax.Const (N_of_ascii "b");
-    FunSyntax.Op FunSyntax.Cons
-    [FunSyntax.Const (N_of_ascii "s");
-    FunSyntax.Op FunSyntax.Cons
-    [FunSyntax.Const (N_of_ascii "s");
-    FunSyntax.Op FunSyntax.Cons
-    [FunSyntax.Const (N_of_ascii "010");
-    FunSyntax.Op FunSyntax.Cons
-    [FunSyntax.Const (N_of_ascii " ");
-    FunSyntax.Op FunSyntax.Cons
-    [FunSyntax.Const (N_of_ascii " "); FunSyntax.Const 0]]]]]]]])
-  (FunSyntax.Const 0))
-).
-Eval lazy in to_cmd (
-  (FunSyntax.Let (FunValues.name_enc "dot_bss")
-  (FunSyntax.Op FunSyntax.Cons
-  [FunSyntax.Const (N_of_ascii "009");
-  FunSyntax.Op FunSyntax.Cons
-  [FunSyntax.Const (N_of_ascii ".");
-  FunSyntax.Op FunSyntax.Cons
-  [FunSyntax.Const (N_of_ascii "b");
-  FunSyntax.Op FunSyntax.Cons
-  [FunSyntax.Const (N_of_ascii "s");
-  FunSyntax.Op FunSyntax.Cons
-  [FunSyntax.Const (N_of_ascii "s");
-  FunSyntax.Op FunSyntax.Cons
-  [FunSyntax.Const (N_of_ascii "010");
-  FunSyntax.Op FunSyntax.Cons
-  [FunSyntax.Const (N_of_ascii " ");
-  FunSyntax.Op FunSyntax.Cons
-  [FunSyntax.Const (N_of_ascii " "); FunSyntax.Const 0]]]]]]]])
-  (FunSyntax.Let (FunValues.name_enc "bss_str") (FunSyntax.Var (FunValues.name_enc "dot_bss"))
-  (FunSyntax.Let (FunValues.name_enc "dot_p2a")
-  (FunSyntax.Op FunSyntax.Cons
-  [FunSyntax.Const (N_of_ascii "009");
-  FunSyntax.Op FunSyntax.Cons
-  [FunSyntax.Const (N_of_ascii ".");
-  FunSyntax.Op FunSyntax.Cons
-  [FunSyntax.Const (N_of_ascii "p");
-  FunSyntax.Op FunSyntax.Cons
-  [FunSyntax.Const (N_of_ascii "2");
-  FunSyntax.Op FunSyntax.Cons
-  [FunSyntax.Const (N_of_ascii "a");
-  FunSyntax.Op FunSyntax.Cons
-  [FunSyntax.Const (N_of_ascii "l");
-  FunSyntax.Op FunSyntax.Cons
-  [FunSyntax.Const (N_of_ascii "i");
-  FunSyntax.Op FunSyntax.Cons
-  [FunSyntax.Const (N_of_ascii "g"); FunSyntax.Const 0]]]]]]]])
-  (FunSyntax.Let (FunValues.name_enc "n3_spc")
-  (FunSyntax.Op FunSyntax.Cons
-  [FunSyntax.Const (N_of_ascii "n");
-  FunSyntax.Op FunSyntax.Cons
-  [FunSyntax.Const (N_of_ascii " ");
-  FunSyntax.Op FunSyntax.Cons
-  [FunSyntax.Const (N_of_ascii "3");
-  FunSyntax.Op FunSyntax.Cons
-  [FunSyntax.Const (N_of_ascii " ");
-  FunSyntax.Op FunSyntax.Cons
-  [FunSyntax.Const (N_of_ascii " ");
-  FunSyntax.Op FunSyntax.Cons
-  [FunSyntax.Const (N_of_ascii " ");
-  FunSyntax.Op FunSyntax.Cons
-  [FunSyntax.Const (N_of_ascii " "); FunSyntax.Const 0]]]]]]])
-  (FunSyntax.Let (FunValues.name_enc "comment1")
-  (FunSyntax.Op FunSyntax.Cons
-  [FunSyntax.Const (N_of_ascii " ");
-  FunSyntax.Op FunSyntax.Cons
-  [FunSyntax.Const (N_of_ascii " ");
-  FunSyntax.Op FunSyntax.Cons
-  [FunSyntax.Const (N_of_ascii " ");
-  FunSyntax.Op FunSyntax.Cons
-  [FunSyntax.Const (N_of_ascii " ");
-  FunSyntax.Op FunSyntax.Cons
-  [FunSyntax.Const (N_of_ascii " ");
-  FunSyntax.Op FunSyntax.Cons
-  [FunSyntax.Const (N_of_ascii " "); FunSyntax.Const 0]]]]]])
-  (FunSyntax.Let (FunValues.name_enc "comment2")
-  (FunSyntax.Op FunSyntax.Cons
-  [FunSyntax.Const (N_of_ascii " ");
-  FunSyntax.Op FunSyntax.Cons
-  [FunSyntax.Const (N_of_ascii " ");
-  FunSyntax.Op FunSyntax.Cons
-  [FunSyntax.Const (N_of_ascii "/");
-  FunSyntax.Op FunSyntax.Cons
-  [FunSyntax.Const (N_of_ascii "*");
-  FunSyntax.Op FunSyntax.Cons
-  [FunSyntax.Const (N_of_ascii " ");
-  FunSyntax.Op FunSyntax.Cons
-  [FunSyntax.Const (N_of_ascii "8");
-  FunSyntax.Op FunSyntax.Cons
-  [FunSyntax.Const (N_of_ascii "-"); FunSyntax.Const 0]]]]]]])
-  (FunSyntax.Let (FunValues.name_enc "comment3")
-  (FunSyntax.Op FunSyntax.Cons
-  [FunSyntax.Const (N_of_ascii "b");
-  FunSyntax.Op FunSyntax.Cons
-  [FunSyntax.Const (N_of_ascii "y");
-  FunSyntax.Op FunSyntax.Cons
-  [FunSyntax.Const (N_of_ascii "t");
-  FunSyntax.Op FunSyntax.Cons
-  [FunSyntax.Const (N_of_ascii "e");
-  FunSyntax.Op FunSyntax.Cons
-  [FunSyntax.Const (N_of_ascii " ");
-  FunSyntax.Op FunSyntax.Cons
-  [FunSyntax.Const (N_of_ascii "a");
-  FunSyntax.Op FunSyntax.Cons
-  [FunSyntax.Const (N_of_ascii "l"); FunSyntax.Const 0]]]]]]])
-  (FunSyntax.Let (FunValues.name_enc "comment4")
-  (FunSyntax.Op FunSyntax.Cons
-  [FunSyntax.Const (N_of_ascii "i");
-  FunSyntax.Op FunSyntax.Cons
-  [FunSyntax.Const (N_of_ascii "g");
-  FunSyntax.Op FunSyntax.Cons
-  [FunSyntax.Const (N_of_ascii "n");
-  FunSyntax.Op FunSyntax.Cons
-  [FunSyntax.Const (N_of_ascii " ");
-  FunSyntax.Op FunSyntax.Cons
-  [FunSyntax.Const (N_of_ascii " ");
-  FunSyntax.Op FunSyntax.Cons
-  [FunSyntax.Const (N_of_ascii " ");
-  FunSyntax.Op FunSyntax.Cons
-  [FunSyntax.Const (N_of_ascii " ");
-  FunSyntax.Const 0]]]]]]])
-  (FunSyntax.Let (FunValues.name_enc "comment5")
-  (FunSyntax.Op FunSyntax.Cons
-  [FunSyntax.Const (N_of_ascii " ");
-  FunSyntax.Op FunSyntax.Cons
-  [FunSyntax.Const (N_of_ascii " ");
-  FunSyntax.Op FunSyntax.Cons
-  [FunSyntax.Const (N_of_ascii " ");
-  FunSyntax.Op FunSyntax.Cons
-  [FunSyntax.Const (N_of_ascii " ");
-  FunSyntax.Op FunSyntax.Cons
-  [FunSyntax.Const (N_of_ascii "*");
-  FunSyntax.Op FunSyntax.Cons
-  [FunSyntax.Const (N_of_ascii "/");
-  FunSyntax.Op FunSyntax.Cons
-  [FunSyntax.Const (N_of_ascii "010");
-  FunSyntax.Op FunSyntax.Cons
-  [FunSyntax.Const (N_of_ascii " ");
-  FunSyntax.Op FunSyntax.Cons
-  [FunSyntax.Const (N_of_ascii " ");
-  FunSyntax.Const 0]]]]]]]]])
-  (FunSyntax.Let (FunValues.name_enc "p2align_temp2")
-  (FunSyntax.Call (FunValues.name_enc "string_append")
-  [FunSyntax.Var (FunValues.name_enc "dot_p2a");
-  FunSyntax.Var (FunValues.name_enc "n3_spc")])
-  (FunSyntax.Let (FunValues.name_enc "p2align_temp3")
-  (FunSyntax.Call (FunValues.name_enc "string_append")
-  [FunSyntax.Var (FunValues.name_enc "p2align_temp2");
-  FunSyntax.Var (FunValues.name_enc "comment1")])
-  (FunSyntax.Let (FunValues.name_enc "p2align_temp4")
-  (FunSyntax.Call (FunValues.name_enc "string_append")
-  [FunSyntax.Var (FunValues.name_enc "p2align_temp3");
-  FunSyntax.Var (FunValues.name_enc "comment2")])
-  (FunSyntax.Let (FunValues.name_enc "p2align_temp5")
-  (FunSyntax.Call (FunValues.name_enc "string_append")
-  [FunSyntax.Var (FunValues.name_enc "p2align_temp4");
-  FunSyntax.Var (FunValues.name_enc "comment3")])
-  (FunSyntax.Let (FunValues.name_enc "p2align_temp6")
-  (FunSyntax.Call (FunValues.name_enc "string_append")
-  [FunSyntax.Var
-  (FunValues.name_enc "p2align_temp5");
-  FunSyntax.Var (FunValues.name_enc "comment4")])
-  (FunSyntax.Let (FunValues.name_enc "p2align_temp7")
   (FunSyntax.Call
-  (FunValues.name_enc "string_append")
-  [FunSyntax.Var
-  (FunValues.name_enc "p2align_temp6");
-  FunSyntax.Var (FunValues.name_enc "comment5")])
-  (FunSyntax.Let (FunValues.name_enc "p2align1_str")
-  (FunSyntax.Var
-  (FunValues.name_enc "p2align_temp7"))
-  (FunSyntax.Let (FunValues.name_enc "heaps_lbl")
-  (FunSyntax.Op FunSyntax.Cons
-  [FunSyntax.Const (N_of_ascii "h");
-  FunSyntax.Op FunSyntax.Cons
-  [FunSyntax.Const (N_of_ascii "e");
-  FunSyntax.Op FunSyntax.Cons
-  [FunSyntax.Const (N_of_ascii "a");
-  FunSyntax.Op FunSyntax.Cons
-  [FunSyntax.Const
-  (N_of_ascii "p");
-  FunSyntax.Op FunSyntax.Cons
-  [FunSyntax.Const
-  (N_of_ascii "S");
-  FunSyntax.Op FunSyntax.Cons
-  [FunSyntax.Const
-  (N_of_ascii ":");
-  FunSyntax.Op
-  FunSyntax.Cons
-  [FunSyntax.Const
-  (N_of_ascii "010");
-  FunSyntax.Op
-  FunSyntax.Cons
-  [FunSyntax.Const
-  (N_of_ascii " ");
-  FunSyntax.Op
-  FunSyntax.Cons
-  [FunSyntax.Const
-  (N_of_ascii
-  " ");
-  FunSyntax.Const
-  0]]]]]]]]])
-  (FunSyntax.Let
-  (FunValues.name_enc "space_cmd")
-  (FunSyntax.Op FunSyntax.Cons
-  [FunSyntax.Const (N_of_ascii "009");
-  FunSyntax.Op FunSyntax.Cons
-  [FunSyntax.Const (N_of_ascii ".");
-  FunSyntax.Op FunSyntax.Cons
-  [FunSyntax.Const
-  (N_of_ascii "s");
-  FunSyntax.Op FunSyntax.Cons
-  [FunSyntax.Const
-  (N_of_ascii "p");
-  FunSyntax.Op FunSyntax.Cons
-  [FunSyntax.Const
-  (N_of_ascii "a");
-  FunSyntax.Op
-  FunSyntax.Cons
-  [FunSyntax.Const
-  (N_of_ascii "c");
-  FunSyntax.Op
-  FunSyntax.Cons
-  [FunSyntax.Const
-  (N_of_ascii "e");
-  FunSyntax.Op
-  FunSyntax.Cons
-  [FunSyntax.Const
-  (N_of_ascii
-  " ");
-  FunSyntax.Const
-  0]]]]]]]])
-  (FunSyntax.Let
-  (FunValues.name_enc "size_str")
-  (FunSyntax.Op FunSyntax.Cons
-  [FunSyntax.Const (N_of_ascii "8");
-  FunSyntax.Op FunSyntax.Cons
-  [FunSyntax.Const
-  (N_of_ascii "*");
-  FunSyntax.Op FunSyntax.Cons
-  [FunSyntax.Const
-  (N_of_ascii "1");
-  FunSyntax.Op FunSyntax.Cons
-  [FunSyntax.Const
-  (N_of_ascii "0");
-  FunSyntax.Op
-  FunSyntax.Cons
-  [FunSyntax.Const
-  (N_of_ascii "2");
-  FunSyntax.Op
-  FunSyntax.Cons
-  [FunSyntax.Const
-  (N_of_ascii "4");
-  FunSyntax.Op
-  FunSyntax.Cons
-  [FunSyntax.Const
-  (N_of_ascii
-  "*");
-  FunSyntax.Const
-  0]]]]]]])
-  (FunSyntax.Let
-  (FunValues.name_enc "size_str2")
-  (FunSyntax.Op FunSyntax.Cons
-  [FunSyntax.Const
-  (N_of_ascii "1");
-  FunSyntax.Op FunSyntax.Cons
-  [FunSyntax.Const
-  (N_of_ascii "0");
-  FunSyntax.Op FunSyntax.Cons
-  [FunSyntax.Const
-  (N_of_ascii "2");
-  FunSyntax.Op
-  FunSyntax.Cons
-  [FunSyntax.Const
-  (N_of_ascii "4");
-  FunSyntax.Op
-  FunSyntax.Cons
-  [FunSyntax.Const
-  (N_of_ascii " ");
-  FunSyntax.Op
-  FunSyntax.Cons
-  [FunSyntax.Const
-  (N_of_ascii
-  " ");
-  FunSyntax.Op
-  FunSyntax.Cons
-  [FunSyntax.Const
-  (N_of_ascii
-  "/");
-  FunSyntax.Const
-  0]]]]]]])
-  (FunSyntax.Let
-  (FunValues.name_enc "comment6")
-  (FunSyntax.Op FunSyntax.Cons
-  [FunSyntax.Const
-  (N_of_ascii "*");
-  FunSyntax.Op FunSyntax.Cons
-  [FunSyntax.Const
-  (N_of_ascii " ");
-  FunSyntax.Op
-  FunSyntax.Cons
-  [FunSyntax.Const
-  (N_of_ascii "b");
-  FunSyntax.Op
-  FunSyntax.Cons
-  [FunSyntax.Const
-  (N_of_ascii "y");
-  FunSyntax.Op
-  FunSyntax.Cons
-  [FunSyntax.Const
-  (N_of_ascii
-  "t");
-  FunSyntax.Op
-  FunSyntax.Cons
-  [FunSyntax.Const
-  (N_of_ascii
-  "e");
-  FunSyntax.Op
-  FunSyntax.Cons
-  [FunSyntax.Const
-  (N_of_ascii
-  "s");
-  FunSyntax.Const
-  0]]]]]]])
-  (FunSyntax.Let
-  (FunValues.name_enc
-  "comment7")
-  (FunSyntax.Op FunSyntax.Cons
-  [FunSyntax.Const
-  (N_of_ascii " ");
-  FunSyntax.Op
-  FunSyntax.Cons
-  [FunSyntax.Const
-  (N_of_ascii "o");
-  FunSyntax.Op
-  FunSyntax.Cons
-  [FunSyntax.Const
-  (N_of_ascii "f");
-  FunSyntax.Op
-  FunSyntax.Cons
-  [FunSyntax.Const
-  (N_of_ascii
-  " ");
-  FunSyntax.Op
-  FunSyntax.Cons
-  [FunSyntax.Const
-  (N_of_ascii
-  "h");
-  FunSyntax.Op
-  FunSyntax.Cons
-  [FunSyntax.Const
-  (N_of_ascii
-  "e");
-  FunSyntax.Op
-  FunSyntax.Cons
-  [FunSyntax.Const
-  (N_of_ascii
-  "a");
-  FunSyntax.Const
-  0]]]]]]])
-  (FunSyntax.Let
-  (FunValues.name_enc
-  "comment8")
-  (FunSyntax.Op
-  FunSyntax.Cons
-  [FunSyntax.Const
-  (N_of_ascii "p");
-  FunSyntax.Op
-  FunSyntax.Cons
-  [FunSyntax.Const
-  (N_of_ascii " ");
-  FunSyntax.Op
-  FunSyntax.Cons
-  [FunSyntax.Const
-  (N_of_ascii
-  "s");
-  FunSyntax.Op
-  FunSyntax.Cons
-  [FunSyntax.Const
-  (N_of_ascii
-  "p");
-  FunSyntax.Op
-  FunSyntax.Cons
-  [FunSyntax.Const
-  (N_of_ascii
-  "a");
-  FunSyntax.Op
-  FunSyntax.Cons
-  [FunSyntax.Const
-  (N_of_ascii
-  "c");
-  FunSyntax.Op
-  FunSyntax.Cons
-  [FunSyntax.Const
-  (N_of_ascii
-  "e");
-  FunSyntax.Const
-  0]]]]]]])
-  (FunSyntax.Let
-  (FunValues.name_enc
-  "comment9")
-  (FunSyntax.Op
-  FunSyntax.Cons
-  [FunSyntax.Const
-  (N_of_ascii " ");
-  FunSyntax.Op
-  FunSyntax.Cons
-  [FunSyntax.Const
-  (N_of_ascii
-  "*");
-  FunSyntax.Op
-  FunSyntax.Cons
-  [FunSyntax.Const
-  (N_of_ascii
-  "/");
-  FunSyntax.Op
-  FunSyntax.Cons
-  [FunSyntax.Const
-  (N_of_ascii
-  "010");
-  FunSyntax.Op
-  FunSyntax.Cons
-  [FunSyntax.Const
-  (N_of_ascii
-  " ");
-  FunSyntax.Op
-  FunSyntax.Cons
-  [FunSyntax.Const
-  (N_of_ascii
-  " ");
-  FunSyntax.Const
-  0]]]]]])
-  (FunSyntax.Let
-  (FunValues.name_enc
-  "space_temp2")
-  (FunSyntax.Call
-  (FunValues.name_enc
-  "string_append")
-  [FunSyntax.Var
-  (FunValues.name_enc
-  "space_cmd");
-  FunSyntax.Var
-  (FunValues.name_enc
-  "size_str")])
-  (FunSyntax.Let
-  (FunValues.name_enc
-  "space_temp3")
-  (FunSyntax.Call
-  (FunValues.name_enc
-  "string_append")
-  [FunSyntax.Var
-  (FunValues.name_enc
-  "space_temp2");
-  FunSyntax.Var
-  (FunValues.name_enc
-  "size_str2")])
-  (FunSyntax.Let
-  (FunValues.name_enc
-  "space_temp4")
-  (FunSyntax.Call
-  (FunValues.name_enc
-  "string_append")
-  [FunSyntax.Var
-  (FunValues.name_enc
-  "space_temp3");
-  FunSyntax.Var
-  (FunValues.name_enc
-  "comment6")])
-  (FunSyntax.Let
-  (FunValues.name_enc
-  "space_temp5")
-  (FunSyntax.Call
-  (FunValues.name_enc
-  "string_append")
-  [FunSyntax.Var
-  (FunValues.name_enc
-  "space_temp4");
-  FunSyntax.Var
-  (FunValues.name_enc
-  "comment7")])
-  (FunSyntax.Let
-  (FunValues.name_enc
-  "space_temp6")
-  (FunSyntax.Call
-  (FunValues.name_enc
-  "string_append")
-  [FunSyntax.Var
-  (FunValues.name_enc
-  "space_temp5");
-  FunSyntax.Var
-  (FunValues.name_enc
-  "comment8")])
-  (FunSyntax.Let
-  (FunValues.name_enc
-  "space_temp7")
-  (FunSyntax.Call
-  (FunValues.name_enc
-  "string_append")
-  [FunSyntax.Var
-  (FunValues.name_enc
-  "space_temp6");
-  FunSyntax.Var
-  (FunValues.name_enc
-  "comment9")])
-  (FunSyntax.Let
-  (FunValues.name_enc
-  "space_str")
-  (FunSyntax.Var
-  (FunValues.name_enc
-  "space_temp7"))
-  (FunSyntax.Let
-  (FunValues.name_enc
-  "list1")
-  (FunSyntax.Op
-  FunSyntax.Cons
-  [FunSyntax.Var
-  (FunValues.name_enc
-  "bss_str");
-  FunSyntax.Op
-  FunSyntax.Cons
-  [FunSyntax.Var
-  (FunValues.name_enc
-  "p2align1_str");
-  FunSyntax.Op
-  FunSyntax.Cons
-  [FunSyntax.Var
-  (FunValues.name_enc
-  "heaps_lbl");
-  FunSyntax.Op
-  FunSyntax.Cons
-  [FunSyntax.Var
-  (FunValues.name_enc
-  "space_str");
-  FunSyntax.Const
-  0]]]])
-  (FunSyntax.Var
-  (FunValues.name_enc
-  "list1"))))))))))))))))))))))))))))))))))
+  (FunValues.name_enc "vel0")
+  [FunSyntax.Op
+    FunSyntax.Cons
+    [FunSyntax.Const
+      (FunValues.name_enc "Pair");
+      FunSyntax.Op
+      FunSyntax.Cons
+      [FunSyntax.Var
+      (FunValues.name_enc "v1");
+      FunSyntax.Op
+      FunSyntax.Cons
+      [FunSyntax.Op
+      FunSyntax.Cons
+      [FunSyntax.Const
+      (FunValues.name_enc "Pair");
+      FunSyntax.Op
+      FunSyntax.Cons
+      [FunSyntax.Var
+      (FunValues.name_enc "v3");
+      FunSyntax.Op
+      FunSyntax.Cons
+      [FunSyntax.Op
+      FunSyntax.Cons
+      [FunSyntax.Const
+      (FunValues.name_enc "Pair");
+      FunSyntax.Op
+      FunSyntax.Cons
+      [FunSyntax.Var
+      (FunValues.name_enc "v5");
+      FunSyntax.Op
+      FunSyntax.Cons
+      [FunSyntax.Var
+      (FunValues.name_enc "v6");
+      FunSyntax.Const 0]]];
+      FunSyntax.Const 0]]];
+    FunSyntax.Const 0]]]
+  ]
+  )
 ).
 
-Eval lazy in compiler_funs_imp.
+Eval lazy in compiler_funs_imp. *)
 
 (* Eval lazy in to_imp compiler_program_prog. *)
