coq/theories/derivations/AsmToStringDerivations.v
@@ -270,38 +270,38 @@ Proof.
 Qed.
 
 Definition ASMToString_funs := [
-  reg2str1_prog;           (* 0 *)
-  lab_prog;                (* 1 *)
-  clean_prog;              (* 2 *)
-  inst2str_prog;           (* 4 *)
-  instrs2str_prog;         (* 5 *)
-  concat_strings_prog;     (* 6 *)
-  asm2str_prog;            (* 7 *)
-  asm2str_header1_prog;    (* 8 *)
-  asm2str_header2_prog;    (* 9 *)
-  asm2str_header3_prog;    (* 10 *)
-  inst2str_const_prog;     (* 11 *)
-  inst2str_mov_prog;       (* 12 *)
-  inst2str_add_prog;       (* 13 *)
-  inst2str_sub_prog;       (* 14 *)
-  inst2str_div_prog;       (* 15 *)
-  inst2str_jump_always_prog; (* 16 *)
-  inst2str_jump_equal_prog; (* 17 *)
-  inst2str_jump_less_prog; (* 18 *)
-  inst2str_call_prog;      (* 19 *)
-  inst2str_ret_prog;       (* 20 *)
-  inst2str_pop_prog;       (* 21 *)
-  inst2str_push_prog;      (* 22 *)
-  inst2str_load_rsp_prog;  (* 23 *)
-  inst2str_store_rsp_prog; (* 24 *)
-  inst2str_add_rsp_prog;   (* 25 *)
-  inst2str_sub_rsp_prog;   (* 26 *)
-  inst2str_store_prog;     (* 27 *)
-  inst2str_load_prog;      (* 28 *)
-  inst2str_getchar1_prog;  (* 29 *)
-  inst2str_putchar_prog;   (* 30 *)
-  inst2str_exit_prog;      (* 31 *)
-  inst2str_comment_prog    (* 32 *)
+  reg2str1_prog;
+  lab_prog;
+  clean_prog;
+  inst2str_const_prog;
+  inst2str_mov_prog;
+  inst2str_add_prog;
+  inst2str_sub_prog;
+  inst2str_div_prog;
+  inst2str_jump_always_prog;
+  inst2str_jump_equal_prog;
+  inst2str_jump_less_prog;
+  inst2str_call_prog;
+  inst2str_ret_prog;
+  inst2str_pop_prog;
+  inst2str_push_prog;
+  inst2str_load_rsp_prog;
+  inst2str_store_rsp_prog;
+  inst2str_add_rsp_prog;
+  inst2str_sub_rsp_prog;
+  inst2str_store_prog;
+  inst2str_load_prog;
+  inst2str_getchar1_prog;
+  inst2str_putchar_prog;
+  inst2str_exit_prog;
+  inst2str_comment_prog;
+  inst2str_prog;
+  instrs2str_prog;
+  concat_strings_prog;
+  asm2str_header1_prog;
+  asm2str_header2_prog;
+  asm2str_header3_prog;
+  asm2str_prog
 ].
 
 Ltac2 assert_eval_app (fname: constr) :=
@@ -339,295 +339,43 @@ Proof.
   assert_eval_app_by 'num2str 'num2str_prog_proof 'Hlookup_fun_utils 6.
   assert_eval_app_by 'N2str_f 'N2str_f_prog_proof 'Hlookup_fun_utils 7.
   assert_eval_app_by 'N2str 'N2str_prog_proof 'Hlookup_fun_utils 8.
-  assert_eval_app_by 'list_length 'list_length_prog_proof 'Hlookup_fun_utils 9.
-  assert_eval_app_by 'list_append 'list_append_prog_proof 'Hlookup_fun_utils 10.
-  assert_eval_app_by 'flatten 'flatten_prog_proof 'Hlookup_fun_utils 11.
-  assert_eval_app_by 'app_list_length 'app_list_length_prog_proof 'Hlookup_fun_utils 12.
+  assert_eval_app_by '@list_length 'list_length_prog_proof 'Hlookup_fun_utils 9.
+  assert_eval_app_by '@list_append 'list_append_prog_proof 'Hlookup_fun_utils 10.
+  assert_eval_app_by '@flatten 'flatten_prog_proof 'Hlookup_fun_utils 11.
+  assert_eval_app_by '@app_list_length 'app_list_length_prog_proof 'Hlookup_fun_utils 12.
   assert_eval_app_by 'string_append 'string_append_prog_proof 'Hlookup_fun_utils 13.
-  assert_eval_app_by 'mul_nat 'mul_nat_prog_proof 'Hlookup_fun_utils 14.
 
-
-
-  assert_eval_app 'reg2str1.
-  1: {
-    eapply reg2str1_prog_proof; eauto; try reflexivity.
-    eapply Hlookup_fun; do 0 (eapply in_cons); eapply in_eq.
-  }
-  assert_eval_app 'lab.
-  1: {
-    eapply lab_prog_proof; eauto; try reflexivity.
-    eapply Hlookup_fun; do 1 (eapply in_cons); eapply in_eq.
-  }
-  assert_eval_app 'clean.
-  1: {
-    eapply clean_prog_proof; eauto; try reflexivity.
-    eapply Hlookup_fun; do 2 (eapply in_cons); eapply in_eq.
-  }
-  assert_eval_app 'inst2str.
-  1: {
-    eapply inst2str_prog_proof; eauto; try reflexivity.
-    eapply Hlookup_fun; do 4 (eapply in_cons); eapply in_eq.
-  }
-  assert_eval_app 'instrs2str.
-  1: {
-    eapply instrs2str_prog_proof; eauto; try reflexivity.
-    eapply Hlookup_fun; do 5 (eapply in_cons); eapply in_eq.
-  }
-  assert_eval_app 'concat_strings.
-  1: {
-    eapply concat_strings_prog_proof; eauto; try reflexivity.
-    eapply Hlookup_fun; do 6 (eapply in_cons); eapply in_eq.
-  }
-  assert_eval_app 'asm2str.
-  1: {
-    eapply asm2str_prog_proof; eauto; try reflexivity.
-    eapply Hlookup_fun; do 7 (eapply in_cons); eapply in_eq.
-  }
-  assert_eval_app 'asm2str_header1.
-  1: {
-    eapply asm2str_header1_prog_proof; eauto; try reflexivity.
-    eapply Hlookup_fun; do 8 (eapply in_cons); eapply in_eq.
-  }
-  assert_eval_app 'asm2str_header2.
-  1: {
-    eapply asm2str_header2_prog_proof; eauto; try reflexivity.
-    eapply Hlookup_fun; do 9 (eapply in_cons); eapply in_eq.
-  }
-  assert_eval_app 'asm2str_header3.
-  1: {
-    eapply asm2str_header3_prog_proof; eauto; try reflexivity.
-    eapply Hlookup_fun; do 10 (eapply in_cons); eapply in_eq.
-  }
-  assert_eval_app 'inst2str_const.
-  1: {
-    eapply inst2str_const_prog_proof; eauto; try reflexivity.
-    eapply Hlookup_fun; do 11 (eapply in_cons); eapply in_eq.
-  }
-  assert_eval_app 'inst2str_mov.
-  1: {
-    eapply inst2str_mov_prog_proof; eauto; try reflexivity.
-    eapply Hlookup_fun; do 12 (eapply in_cons); eapply in_eq.
-  }
-  assert_eval_app 'inst2str_add.
-  1: {
-    eapply inst2str_add_prog_proof; eauto; try reflexivity.
-    eapply Hlookup_fun; do 13 (eapply in_cons); eapply in_eq.
-  }
-  assert_eval_app 'inst2str_sub.
-  1: {
-    eapply inst2str_sub_prog_proof; eauto; try reflexivity.
-    eapply Hlookup_fun; do 14 (eapply in_cons); eapply in_eq.
-  }
-  assert_eval_app 'inst2str_div.
-  1: {
-    eapply inst2str_div_prog_proof; eauto; try reflexivity.
-    eapply Hlookup_fun; do 15 (eapply in_cons); eapply in_eq.
-  }
-  assert_eval_app 'inst2str_jump_always.
-  1: {
-    eapply inst2str_jump_always_prog_proof; eauto; try reflexivity.
-    eapply Hlookup_fun; do 16 (eapply in_cons); eapply in_eq.
-  }
-  assert_eval_app 'inst2str_jump_equal.
-  1: {
-    eapply inst2str_jump_equal_prog_proof; eauto; try reflexivity.
-    eapply Hlookup_fun; do 17 (eapply in_cons); eapply in_eq.
-  }
-  assert_eval_app 'inst2str_jump_less.
-  1: {
-    eapply inst2str_jump_less_prog_proof; eauto; try reflexivity.
-    eapply Hlookup_fun; do 18 (eapply in_cons); eapply in_eq.
-  }
-  assert_eval_app 'inst2str_call.
-  1: {
-    eapply inst2str_call_prog_proof; eauto; try reflexivity.
-    eapply Hlookup_fun; do 19 (eapply in_cons); eapply in_eq.
-  }
-  assert_eval_app 'inst2str_ret.
-  1: {
-    eapply inst2str_ret_prog_proof; eauto; try reflexivity.
-    eapply Hlookup_fun; do 20 (eapply in_cons); eapply in_eq.
-  }
-  assert_eval_app 'inst2str_pop.
-  1: {
-    eapply inst2str_pop_prog_proof; eauto; try reflexivity.
-    eapply Hlookup_fun; do 21 (eapply in_cons); eapply in_eq.
-  }
-  assert_eval_app 'inst2str_push.
-  1: {
-    eapply inst2str_push_prog_proof; eauto; try reflexivity.
-    eapply Hlookup_fun; do 22 (eapply in_cons); eapply in_eq.
-  }
-  assert_eval_app 'inst2str_load_rsp.
-  1: {
-    eapply inst2str_load_rsp_prog_proof; eauto; try reflexivity.
-    eapply Hlookup_fun; do 23 (eapply in_cons); eapply in_eq.
-  }
-  assert_eval_app 'inst2str_store_rsp.
-  1: {
-    eapply inst2str_store_rsp_prog_proof; eauto; try reflexivity.
-    eapply Hlookup_fun; do 24 (eapply in_cons); eapply in_eq.
-  }
-  assert_eval_app 'inst2str_add_rsp.
-  1: {
-    eapply inst2str_add_rsp_prog_proof; eauto; try reflexivity.
-    eapply Hlookup_fun; do 25 (eapply in_cons); eapply in_eq.
-  }
-  assert_eval_app 'inst2str_sub_rsp.
-  1: {
-    eapply inst2str_sub_rsp_prog_proof; eauto; try reflexivity.
-    eapply Hlookup_fun; do 26 (eapply in_cons); eapply in_eq.
-  }
-  assert_eval_app 'inst2str_store.
-  1: {
-    eapply inst2str_store_prog_proof; eauto; try reflexivity.
-    eapply Hlookup_fun; do 27 (eapply in_cons); eapply in_eq.
-  }
-  assert_eval_app 'inst2str_load.
-  1: {
-    eapply inst2str_load_prog_proof; eauto; try reflexivity.
-    eapply Hlookup_fun; do 28 (eapply in_cons); eapply in_eq.
-  }
-  assert_eval_app 'inst2str_getchar1.
-  1: {
-    eapply inst2str_getchar1_prog_proof; eauto; try reflexivity.
-    eapply Hlookup_fun; do 29 (eapply in_cons); eapply in_eq.
-  }
-  assert_eval_app 'inst2str_putchar.
-  1: {
-    eapply inst2str_putchar_prog_proof; eauto; try reflexivity.
-    eapply Hlookup_fun; do 30 (eapply in_cons); eapply in_eq.
-  }
-  assert_eval_app 'inst2str_exit.
-  1: {
-    eapply inst2str_exit_prog_proof; eauto; try reflexivity.
-    eapply Hlookup_fun; do 31 (eapply in_cons); eapply in_eq.
-  }
-  assert_eval_app 'inst2str_comment.
-  1: {
-    eapply inst2str_comment_prog_proof; eauto; try reflexivity.
-    eapply Hlookup_fun; do 32 (eapply in_cons); eapply in_eq.
-  }
-
-  assert_eval_app '@list_append.
-  1: {
-    eapply list_append_prog_proof; eauto; try reflexivity.
-    eapply Hlookup_fun; do 40 (eapply in_cons); eapply in_eq.
-  }
-  assert_eval_app 'string_append.
-  1: {
-    eapply string_append_prog_proof; eauto; try reflexivity.
-    eapply Hlookup_fun; do 3 (eapply in_cons); eapply in_eq.
-  }
-  assert_eval_app 'mul_N.
-  1: {
-    eapply mul_N_prog_proof; eauto; try reflexivity.
-    2: eapply Hlookup_fun; do 45 (eapply in_cons); eapply in_eq.
-    eapply mul_N_f_prog_proof; eauto; try reflexivity.
-    eapply Hlookup_fun; do 44 (eapply in_cons); eapply in_eq.
-  }
-  assert_eval_app 'mul_nat.
-  1: {
-    eapply mul_nat_prog_proof; eauto; try reflexivity.
-    eapply Hlookup_fun; do 43 (eapply in_cons); eapply in_eq.
-  }
-  assert_eval_app 'num2str.
-  1: {
-    eapply num2str_prog_proof; eauto; try reflexivity.
-    2: eapply Hlookup_fun; do 36 (eapply in_cons); eapply in_eq.
-    eapply num2str_f_prog_proof; eauto; try reflexivity.
-    2: eapply Hlookup_fun; do 35 (eapply in_cons); eapply in_eq.
-    eapply nat_modulo_prog_proof; eauto; try reflexivity.
-    eapply Hlookup_fun; do 33 (eapply in_cons); eapply in_eq.
-  }
-  assert_eval_app 'concat_strings.
-  1: {
-    eapply concat_strings_prog_proof; eauto; try reflexivity.
-    eapply Hlookup_fun; do 6 (eapply in_cons); eapply in_eq.
-  }
-  assert_eval_app 'string_append.
-  1: {
-    eapply string_append_prog_proof; eauto; try reflexivity.
-    eapply Hlookup_fun; do 3 (eapply in_cons); eapply in_eq.
-  }
-  assert_eval_app 'reg2str1.
-  1: {
-    eapply reg2str1_prog_proof; eauto; try reflexivity.
-    eapply Hlookup_fun; do 0 (eapply in_cons); eapply in_eq.
-  }
-  assert_eval_app 'N2str.
-  1: {
-    eapply N2str_prog_proof; eauto; try reflexivity.
-    2: eapply Hlookup_fun; do 38 (eapply in_cons); eapply in_eq.
-    eapply N2str_f_prog_proof; eauto; try reflexivity.
-    2: eapply Hlookup_fun; do 37 (eapply in_cons); eapply in_eq.
-    eapply N_modulo_prog_proof; eauto; try reflexivity.
-    eapply Hlookup_fun; do 34 (eapply in_cons); eapply in_eq.
-  }
-  assert_eval_app 'lab.
-  1: {
-    eapply lab_prog_proof; eauto; try reflexivity.
-    eapply Hlookup_fun; do 1 (eapply in_cons); eapply in_eq.
-  }
-  assert_eval_app 'instrs2str.
-  1: {
-    eapply instrs2str_prog_proof; eauto; try reflexivity.
-    2: eapply Hlookup_fun; do 5 (eapply in_cons); eapply in_eq.
-    eapply inst2str_prog_proof; eauto; try reflexivity.
-    23: eapply Hlookup_fun; do 4 (eapply in_cons); eapply in_eq.
-    1: eapply inst2str_const_prog_proof; eauto; try reflexivity.
-    1: eapply Hlookup_fun; do 11 (eapply in_cons); eapply in_eq.
-    1: eapply inst2str_mov_prog_proof; eauto; try reflexivity.
-    1: eapply Hlookup_fun; do 12 (eapply in_cons); eapply in_eq.
-    1: eapply inst2str_add_prog_proof; eauto; try reflexivity.
-    1: eapply Hlookup_fun; do 13 (eapply in_cons); eapply in_eq.
-    1: eapply inst2str_sub_prog_proof; eauto; try reflexivity.
-    1: eapply Hlookup_fun; do 14 (eapply in_cons); eapply in_eq.
-    1: eapply inst2str_div_prog_proof; eauto; try reflexivity.
-    1: eapply Hlookup_fun; do 15 (eapply in_cons); eapply in_eq.
-    1: eapply inst2str_jump_always_prog_proof; eauto; try reflexivity.
-    1: eapply Hlookup_fun; do 16 (eapply in_cons); eapply in_eq.
-    1: eapply inst2str_jump_equal_prog_proof; eauto; try reflexivity.
-    1: eapply Hlookup_fun; do 17 (eapply in_cons); eapply in_eq.
-    1: eapply inst2str_jump_less_prog_proof; eauto; try reflexivity.
-    1: eapply Hlookup_fun; do 18 (eapply in_cons); eapply in_eq.
-    1: eapply inst2str_call_prog_proof; eauto; try reflexivity.
-    1: eapply Hlookup_fun; do 19 (eapply in_cons); eapply in_eq.
-    1: eapply inst2str_ret_prog_proof; eauto; try reflexivity.
-    1: eapply Hlookup_fun; do 20 (eapply in_cons); eapply in_eq.
-    1: eapply inst2str_pop_prog_proof; eauto; try reflexivity.
-    1: eapply Hlookup_fun; do 21 (eapply in_cons); eapply in_eq.
-    1: eapply inst2str_push_prog_proof; eauto; try reflexivity.
-    1: eapply Hlookup_fun; do 22 (eapply in_cons); eapply in_eq.
-    1: eapply inst2str_load_rsp_prog_proof; eauto; try reflexivity.
-    1: eapply Hlookup_fun; do 23 (eapply in_cons); eapply in_eq.
-    1: eapply inst2str_store_rsp_prog_proof; eauto; try reflexivity.
-    1: eapply Hlookup_fun; do 24 (eapply in_cons); eapply in_eq.
-    1: eapply inst2str_add_rsp_prog_proof; eauto; try reflexivity.
-    1: eapply Hlookup_fun; do 25 (eapply in_cons); eapply in_eq.
-    1: eapply inst2str_sub_rsp_prog_proof; eauto; try reflexivity.
-    1: eapply Hlookup_fun; do 26 (eapply in_cons); eapply in_eq.
-    1: eapply inst2str_store_prog_proof; eauto; try reflexivity.
-    1: eapply Hlookup_fun; do 27 (eapply in_cons); eapply in_eq.
-    1: eapply inst2str_load_prog_proof; eauto; try reflexivity.
-    1: eapply Hlookup_fun; do 28 (eapply in_cons); eapply in_eq.
-    1: eapply inst2str_getchar1_prog_proof; eauto; try reflexivity.
-    1: eapply Hlookup_fun; do 29 (eapply in_cons); eapply in_eq.
-    1: eapply inst2str_putchar_prog_proof; eauto; try reflexivity.
-    1: eapply Hlookup_fun; do 30 (eapply in_cons); eapply in_eq.
-    1: eapply inst2str_exit_prog_proof; eauto; try reflexivity.
-    1: eapply Hlookup_fun; do 31 (eapply in_cons); eapply in_eq.
-    eapply inst2str_comment_prog_proof; eauto; try reflexivity.
-    2: eapply Hlookup_fun; do 32 (eapply in_cons); eapply in_eq.
-    eapply clean_prog_proof; eauto; try reflexivity.
-    eapply Hlookup_fun; do 2 (eapply in_cons); eapply in_eq.
-  }
-  eapply asm2str_prog_proof; eauto; try reflexivity.
-  4: eapply Hlookup_fun; do 7 (eapply in_cons); eapply in_eq.
-  1: eapply asm2str_header1_prog_proof; eauto; try reflexivity.
-  1: eapply Hlookup_fun; do 8 (eapply in_cons); eapply in_eq.
-  1: eapply asm2str_header2_prog_proof; eauto; try reflexivity.
-  1: eapply Hlookup_fun; do 9 (eapply in_cons); eapply in_eq.
-  eapply asm2str_header3_prog_proof; eauto; try reflexivity.
-  eapply Hlookup_fun; do 10 (eapply in_cons); eapply in_eq.
+  assert_eval_app_by 'reg2str1 'reg2str1_prog_proof 'Hlookup_fun 0.
+  assert_eval_app_by 'lab 'lab_prog_proof 'Hlookup_fun 1.
+  assert_eval_app_by 'clean 'clean_prog_proof 'Hlookup_fun 2.
+  assert_eval_app_by 'inst2str_const 'inst2str_const_prog_proof 'Hlookup_fun 3.
+  assert_eval_app_by 'inst2str_mov 'inst2str_mov_prog_proof 'Hlookup_fun 4.
+  assert_eval_app_by 'inst2str_add 'inst2str_add_prog_proof 'Hlookup_fun 5.
+  assert_eval_app_by 'inst2str_sub 'inst2str_sub_prog_proof 'Hlookup_fun 6.
+  assert_eval_app_by 'inst2str_div 'inst2str_div_prog_proof 'Hlookup_fun 7.
+  assert_eval_app_by 'inst2str_jump_always 'inst2str_jump_always_prog_proof 'Hlookup_fun 8.
+  assert_eval_app_by 'inst2str_jump_equal 'inst2str_jump_equal_prog_proof 'Hlookup_fun 9.
+  assert_eval_app_by 'inst2str_jump_less 'inst2str_jump_less_prog_proof 'Hlookup_fun 10.
+  assert_eval_app_by 'inst2str_call 'inst2str_call_prog_proof 'Hlookup_fun 11.
+  assert_eval_app_by 'inst2str_ret 'inst2str_ret_prog_proof 'Hlookup_fun 12.
+  assert_eval_app_by 'inst2str_pop 'inst2str_pop_prog_proof 'Hlookup_fun 13.
+  assert_eval_app_by 'inst2str_push 'inst2str_push_prog_proof 'Hlookup_fun 14.
+  assert_eval_app_by 'inst2str_load_rsp 'inst2str_load_rsp_prog_proof 'Hlookup_fun 15.
+  assert_eval_app_by 'inst2str_store_rsp 'inst2str_store_rsp_prog_proof 'Hlookup_fun 16.
+  assert_eval_app_by 'inst2str_add_rsp 'inst2str_add_rsp_prog_proof 'Hlookup_fun 17.
+  assert_eval_app_by 'inst2str_sub_rsp 'inst2str_sub_rsp_prog_proof 'Hlookup_fun 18.
+  assert_eval_app_by 'inst2str_store 'inst2str_store_prog_proof 'Hlookup_fun 19.
+  assert_eval_app_by 'inst2str_load 'inst2str_load_prog_proof 'Hlookup_fun 20.
+  assert_eval_app_by 'inst2str_getchar1 'inst2str_getchar1_prog_proof 'Hlookup_fun 21.
+  assert_eval_app_by 'inst2str_putchar 'inst2str_putchar_prog_proof 'Hlookup_fun 22.
+  assert_eval_app_by 'inst2str_exit 'inst2str_exit_prog_proof 'Hlookup_fun 23.
+  assert_eval_app_by 'inst2str_comment 'inst2str_comment_prog_proof 'Hlookup_fun 24.
+  assert_eval_app_by 'inst2str 'inst2str_prog_proof 'Hlookup_fun 25.
+  assert_eval_app_by 'instrs2str 'instrs2str_prog_proof 'Hlookup_fun 26.
+  assert_eval_app_by 'concat_strings 'concat_strings_prog_proof 'Hlookup_fun 27.
+  assert_eval_app_by 'asm2str_header1 'asm2str_header1_prog_proof 'Hlookup_fun 28.
+  assert_eval_app_by 'asm2str_header2 'asm2str_header2_prog_proof 'Hlookup_fun 29.
+  assert_eval_app_by 'asm2str_header3 'asm2str_header3_prog_proof 'Hlookup_fun 30.
+  assert_eval_app_by 'asm2str 'asm2str_prog_proof 'Hlookup_fun 31.
+  eauto.
 Qed.
